checkpoint; actions in msttot

ulib/experimental/Steel.PCM.Memory.fst
@@ -167,10 +167,10 @@ let affine_star (p q:slprop) (m:mem) =
 // Invariants on the lock store
 ////////////////////////////////////////////////////////////////////////////////
 
-let lock_addr = nat
+let iname = nat
 module S = FStar.Set
 module L = FStar.List.Tot
-let rec lock_store_invariant (e:S.set lock_addr) (l:lock_store u#a) : slprop u#a =
+let rec lock_store_invariant (e:inames) (l:lock_store u#a) : slprop u#a =
   let current_addr = L.length l - 1 in
   match l with
   | [] -> emp
@@ -183,7 +183,7 @@ let rec lock_store_invariant (e:S.set lock_addr) (l:lock_store u#a) : slprop u#a
 let heap_ctr_valid (ctr:nat) (h:H.heap u#a) : H.a_heap_prop u#a =
   fun _ -> h `H.free_above_addr` ctr
 
-let locks_invariant (e:S.set lock_addr) (m:mem u#a) : slprop u#a =
+let locks_invariant (e:inames) (m:mem u#a) : slprop u#a =
   H.h_refine (lock_store_invariant e m.locks)
              (heap_ctr_valid m.ctr (heap_of_mem m))
 
@@ -204,58 +204,84 @@ let h_exists_cong (#a:Type) (p q : a -> slprop)
 // Lifting heap actions
 ////////////////////////////////////////////////////////////////////////////////
 
-let linv (m:mem) = locks_invariant Set.empty m
+let tot_pre_action_except (e:inames) (fp:slprop u#a) (a:Type u#b) (fp':a -> slprop u#a) =
+  hmem_with_inv_except e fp -> (x:a & hmem_with_inv_except e (fp' x))
 
-let hheap_of_hmem #fp (m:hmem_with_inv fp)
-  : h:H.hheap (fp `star` linv m) { h `H.free_above_addr` m.ctr}
-  = let h = heap_of_mem m in
-    H.refine_interp (lock_store_invariant S.empty m.locks)
-                    (heap_ctr_valid m.ctr (heap_of_mem m)) h;
-    h
+let tot_pre_action = tot_pre_action_except S.empty
 
-let hmem_of_hheap (#fp0 #fp1:slprop) (m:hmem_with_inv fp0)
-                  (h:H.hheap (fp1 `star` linv m) {
-                       h `Heap.free_above_addr` m.ctr
-                  })
-    : m1:hmem_with_inv fp1{linv m `equiv` linv m1}
-    = let m1 : mem = { m with heap = h } in
-      assert (interp (fp1 `star` linv m) m1);
-      star_commutative fp1 (linv m);
-      assert (interp (linv m `star` fp1) m1);
-      assert (linv m1 ==  H.h_refine (lock_store_invariant S.empty m1.locks)
-                                     (heap_ctr_valid m1.ctr (heap_of_mem m1)));
-      assert (linv m ==  H.h_refine (lock_store_invariant S.empty m1.locks)
-                                    (heap_ctr_valid m1.ctr (heap_of_mem m)));
-      H.refine_interp (lock_store_invariant S.empty m1.locks)
-                      (heap_ctr_valid m1.ctr (heap_of_mem m))
-                      (heap_of_mem m);
-      assert (forall h. (heap_ctr_valid m1.ctr (heap_of_mem m)) h <==>
-                   (heap_ctr_valid m1.ctr (heap_of_mem m1)) h);
-      H.refine_equiv (lock_store_invariant S.empty m1.locks)
-                     (lock_store_invariant S.empty m1.locks)
-                     (heap_ctr_valid m1.ctr (heap_of_mem m))
-                     (heap_ctr_valid m1.ctr (heap_of_mem m1));
-      assert (linv m `equiv` linv m1);
-      let _ = equiv_extensional_on_star (linv m) (linv m1) fp1 in
-      assert ((linv m `star` fp1) `equiv` (linv m1 `star` fp1));
-      assert (interp (linv m1 `star` fp1) m1);
-      star_commutative (linv m1) fp1;
-      assert (interp (fp1 `star` linv m1) m1);
-      m1
-
-let ac_reasoning_for_m_frame_preserving p q r m =
-  calc (equiv) {
+let ac_reasoning_for_m_frame_preserving
+    (p q r:slprop u#a) (m:mem u#a)
+  : Lemma
+    (requires interp ((p `star` q) `star` r) m)
+    (ensures interp (p `star` r) m)
+  = calc (equiv) {
     (p `star` q) `star` r;
        (equiv) { star_commutative p q;
                  equiv_extensional_on_star (p `star` q) (q `star` p) r }
     (q `star` p) `star` r;
        (equiv) { star_associative q p r }
     q `star` (p `star` r);
-  };
-  assert (interp (q `star` (p `star` r)) m);
-  affine_star q (p `star` r) m
+    };
+    assert (interp (q `star` (p `star` r)) m);
+    affine_star q (p `star` r) m
 
-let with_inv (m:mem) (fp:slprop) = interp (fp `star` locks_invariant Set.empty m) m
+let is_frame_preserving
+  (#e:inames)
+  (#a:Type u#b)
+  (#fp:slprop u#a)
+  (#fp':a -> slprop u#a)
+  (f:tot_pre_action_except e fp a fp') =
+  forall (frame:slprop u#a) (m0:hmem_with_inv_except e (fp `star` frame)).
+    (ac_reasoning_for_m_frame_preserving fp frame (locks_invariant e m0) m0;
+     let (| x, m1 |) = f m0 in
+     interp ((fp' x `star` frame) `star` locks_invariant e m1) m1 /\
+     (forall (mp:mprop frame). mp (core_mem m0) == mp (core_mem m1)))
+
+let tot_action_except (e:inames) (fp:slprop u#a) (a:Type u#b) (fp':a -> slprop u#a) =
+  f:tot_pre_action_except e fp a fp'{ is_frame_preserving f }
+
+let tot_action = tot_action_except S.empty
+
+let linv e (m:mem) = locks_invariant e m
+
+let hheap_of_hmem #fp #e (m:hmem_with_inv_except e fp)
+  : h:H.hheap (fp `star` linv e m) { h `H.free_above_addr` m.ctr}
+  = let h = heap_of_mem m in
+    H.refine_interp (lock_store_invariant e m.locks)
+                    (heap_ctr_valid m.ctr (heap_of_mem m)) h;
+    h
+
+let hmem_of_hheap #e (#fp0 #fp1:slprop) (m:hmem_with_inv_except e fp0)
+                  (h:H.hheap (fp1 `star` linv e m) {
+                       h `Heap.free_above_addr` m.ctr
+                  })
+    : m1:hmem_with_inv_except e fp1{linv e m `equiv` linv e m1}
+    = let m1 : mem = { m with heap = h } in
+      assert (interp (fp1 `star` linv e m) m1);
+      star_commutative fp1 (linv e m);
+      assert (interp (linv e m `star` fp1) m1);
+      assert (linv e m1 ==  H.h_refine (lock_store_invariant e m1.locks)
+                                       (heap_ctr_valid m1.ctr (heap_of_mem m1)));
+      assert (linv e m ==  H.h_refine (lock_store_invariant e m1.locks)
+                                      (heap_ctr_valid m1.ctr (heap_of_mem m)));
+      H.refine_interp (lock_store_invariant e m1.locks)
+                      (heap_ctr_valid m1.ctr (heap_of_mem m))
+                      (heap_of_mem m);
+      assert (forall h. (heap_ctr_valid m1.ctr (heap_of_mem m)) h <==>
+                   (heap_ctr_valid m1.ctr (heap_of_mem m1)) h);
+      H.refine_equiv (lock_store_invariant e m1.locks)
+                     (lock_store_invariant e m1.locks)
+                     (heap_ctr_valid m1.ctr (heap_of_mem m))
+                     (heap_ctr_valid m1.ctr (heap_of_mem m1));
+      assert (linv e m `equiv` linv e m1);
+      let _ = equiv_extensional_on_star (linv e m) (linv e m1) fp1 in
+      assert ((linv e m `star` fp1) `equiv` (linv e m1 `star` fp1));
+      assert (interp (linv e m1 `star` fp1) m1);
+      star_commutative (linv e m1) fp1;
+      assert (interp (fp1 `star` linv e m1) m1);
+      m1
+
+let with_inv_except (m:mem) e (fp:slprop) = interp (fp `star` locks_invariant e m) m
 
 #push-options "--warn_error -271"
 let as_hprop (frame:slprop) (mp:mprop frame)
@@ -284,35 +310,36 @@ let mprop_preservation_of_hprop_preservation
       ()
 
 let lift_heap_action (#fp:slprop) (#a:Type) (#fp':a -> slprop)
+                     (e:inames)
                      ($f:H.action fp a fp')
-  : action fp a fp'
-  = let g : pre_action fp a fp' = fun m ->
+  : tot_action_except e fp a fp'
+  = let g : tot_pre_action_except e fp a fp' = fun m ->
         let h0 = hheap_of_hmem m in
         let (| x, h' |) = f h0 in
         (| x, hmem_of_hheap m h' |)
     in
-    let aux (frame:slprop) (m0:hmem_with_inv (fp `star` frame))
+    let aux (frame:slprop) (m0:hmem_with_inv_except e (fp `star` frame))
       : Lemma
         (ensures
-          (ac_reasoning_for_m_frame_preserving fp frame (locks_invariant Set.empty m0) m0;
+          (ac_reasoning_for_m_frame_preserving fp frame (locks_invariant e m0) m0;
            let (| x, m1 |) = g m0 in
-           interp ((fp' x `star` frame) `star` locks_invariant Set.empty m1) m1 /\
+           interp ((fp' x `star` frame) `star` locks_invariant e m1) m1 /\
            (forall (mp:mprop frame). mp (core_mem m0) == mp (core_mem m1))))
         [SMTPat ()]
-      = ac_reasoning_for_m_frame_preserving fp frame (locks_invariant Set.empty m0) m0;
+      = ac_reasoning_for_m_frame_preserving fp frame (locks_invariant e m0) m0;
         let (| x, m1 |) = g m0 in
         let h0 = hheap_of_hmem m0 in
         let (| x', h1 |) = f h0 in
-        H.action_framing f (linv m0) h0;
+        H.action_framing f (linv e m0) h0;
         assert (x == x');
-        star_associative fp frame (linv m0);
-        H.action_framing f (frame `star` linv m0) h0;
-        assert (H.interp ((fp' x) `star` (frame `star` linv m0)) h1);
-        star_associative (fp' x) frame (linv m0);
-        assert (H.interp ((fp' x `star` frame) `star` linv m0) h1);
-        let h1' : H.hheap ((fp' x `star` frame) `star` linv m0) = h1 in
+        star_associative fp frame (linv e m0);
+        H.action_framing f (frame `star` linv e m0) h0;
+        assert (H.interp ((fp' x) `star` (frame `star` linv e m0)) h1);
+        star_associative (fp' x) frame (linv e m0);
+        assert (H.interp ((fp' x `star` frame) `star` linv e m0) h1);
+        let h1' : H.hheap ((fp' x `star` frame) `star` linv e m0) = h1 in
         assert (m1 == hmem_of_hheap m0 h1');
-        assert (with_inv m1 (fp' x `star` frame));
+        assert (with_inv_except m1 e (fp' x `star` frame));
         assert (forall (hp:H.hprop frame). hp h0 == hp h1);
         mprop_preservation_of_hprop_preservation frame m0 m1;
         ()
@@ -320,13 +347,20 @@ let lift_heap_action (#fp:slprop) (#a:Type) (#fp':a -> slprop)
     assert (is_frame_preserving g);
     g
 
-let sel_action r v0
-  = lift_heap_action (H.sel_action r v0)
+let mem_evolves = admit()
 
-let upd_action r v0 v1
-  = lift_heap_action (H.upd_action r v0 v1)
+let lift_tot_action #a #e #fp #fp' ($f:tot_action_except e fp a fp')
+  : action_except a e fp fp'
+  = admit()
 
-let free_action r v0 = lift_heap_action (H.free_action r v0)
+let sel_action e r v0
+  = lift_tot_action (lift_heap_action e (H.sel_action r v0))
+
+let upd_action e r v0 v1
+  = lift_tot_action (lift_heap_action e (H.upd_action r v0 v1))
+
+let free_action e r v0
+  = lift_tot_action (lift_heap_action e (H.free_action r v0))
 
 let weaken (p q r:slprop) (h:H.hheap (p `star` q) { H.stronger q r })
   : H.hheap (p `star` r)
@@ -344,92 +378,88 @@ let weaken_refine (p:slprop) (q r:H.a_heap_prop)
     in
     ()
 
-let inc_ctr (#p:slprop) (m:hmem_with_inv p)
-  : m':hmem_with_inv p{m'.ctr = m.ctr + 1 /\ H.stronger (linv m) (linv m')}
+let inc_ctr (#p:slprop) #e (m:hmem_with_inv_except e p)
+  : m':hmem_with_inv_except e p{m'.ctr = m.ctr + 1 /\ H.stronger (linv e m) (linv e m')}
   = let m' : mem = { m with ctr = m.ctr + 1} in
-    assert (interp (p `star` linv m) m');
-    assert (linv m == H.h_refine (lock_store_invariant Set.empty m.locks)
-                                 (heap_ctr_valid m.ctr (heap_of_mem m)));
-    assert (linv m' == H.h_refine (lock_store_invariant Set.empty m.locks)
-                                  (heap_ctr_valid (m.ctr + 1) (heap_of_mem m)));
+    assert (interp (p `star` linv e m) m');
+    assert (linv e m == H.h_refine (lock_store_invariant e m.locks)
+                                   (heap_ctr_valid m.ctr (heap_of_mem m)));
+    assert (linv e m' == H.h_refine (lock_store_invariant e m.locks)
+                                    (heap_ctr_valid (m.ctr + 1) (heap_of_mem m)));
     H.weaken_free_above (heap_of_mem m) m.ctr (m.ctr + 1);
-    weaken_refine (lock_store_invariant Set.empty m.locks)
+    weaken_refine (lock_store_invariant e m.locks)
                   (heap_ctr_valid m.ctr (heap_of_mem m))
                   (heap_ctr_valid (m.ctr + 1) (heap_of_mem m));
-    assert (H.stronger (linv m) (linv m'));
-    let _ = weaken p (linv m) (linv m') (heap_of_mem m) in
+    assert (H.stronger (linv e m) (linv e m'));
+    let _ = weaken p (linv e m) (linv e m') (heap_of_mem m) in
     m'
 
-let frame_related_mems (fp0 fp1:slprop u#a) (m0:hmem_with_inv fp0) (m1:hmem_with_inv fp1) =
+let frame_related_mems (fp0 fp1:slprop u#a) e (m0:hmem_with_inv_except e fp0) (m1:hmem_with_inv_except e fp1) =
     forall (frame:slprop u#a).
-      interp ((fp0 `star` frame) `star` linv m0) m0 ==>
-      interp ((fp1 `star` frame) `star` linv m1) m1 /\
+      interp ((fp0 `star` frame) `star` linv e m0) m0 ==>
+      interp ((fp1 `star` frame) `star` linv e m1) m1 /\
       (forall (mp:mprop frame). mp (core_mem m0) == mp (core_mem m1))
 
-let refined_pre_action (fp0:slprop) (a:Type) (fp1:a -> slprop) =
-  m0:hmem_with_inv fp0 ->
+let refined_pre_action e (fp0:slprop) (a:Type) (fp1:a -> slprop) =
+  m0:hmem_with_inv_except e fp0 ->
   Pure (x:a &
-        hmem_with_inv (fp1 x))
+        hmem_with_inv_except e (fp1 x))
        (requires True)
        (ensures fun  (| x, m1 |) ->
-         frame_related_mems fp0 (fp1 x) m0 m1)
+         frame_related_mems fp0 (fp1 x) e m0 m1)
 
 let refined_pre_action_as_action (#fp0:slprop) (#a:Type) (#fp1:a -> slprop)
-                                 ($f:refined_pre_action fp0 a fp1)
-  : action fp0 a fp1
-  = let g : pre_action fp0 a fp1 = fun m -> f m in
+                                 #e ($f:refined_pre_action e fp0 a fp1)
+  : tot_action_except e fp0 a fp1
+  = let g : tot_pre_action_except e fp0 a fp1 = fun m -> f m in
     let aux (frame:slprop)
-            (m0:hmem_with_inv (fp0 `star` frame))
+            (m0:hmem_with_inv_except e (fp0 `star` frame))
       : Lemma
         (ensures
-          (ac_reasoning_for_m_frame_preserving fp0 frame (locks_invariant Set.empty m0) m0;
+          (ac_reasoning_for_m_frame_preserving fp0 frame (locks_invariant e m0) m0;
            let (| x, m1 |) = g m0 in
-           interp ((fp1 x `star` frame) `star` locks_invariant Set.empty m1) m1 /\
+           interp ((fp1 x `star` frame) `star` locks_invariant e m1) m1 /\
           (forall (mp:mprop frame). mp (core_mem m0) == mp (core_mem m1))))
         [SMTPat ()]
-      = ac_reasoning_for_m_frame_preserving fp0 frame (locks_invariant Set.empty m0) m0;
+      = ac_reasoning_for_m_frame_preserving fp0 frame (locks_invariant e m0) m0;
         let (| x', m1' |) = g m0 in
         let (| x, m1 |) = f m0 in
         assert (x == x' /\ m1 == m1')
     in
     g
 
-let alloc_action (#a:Type u#a) (#pcm:pcm a) (x:a{compatible pcm x x})
-  = let f (m0:hmem_with_inv emp)
-      : Pure (r:ref a pcm &
-              hmem_with_inv (pts_to #a r x))
-             (requires True)
-             (ensures fun  (| r, m1 |) ->
-               frame_related_mems emp (pts_to r x) m0 m1)
-      = let h = hheap_of_hmem m0 in
+let alloc_action #a #pcm e x
+  = let f : refined_pre_action e emp (ref a pcm) (fun r -> pts_to r x)
+      = fun m0 ->
+        let h = hheap_of_hmem m0 in
         let (|r, h'|) = H.extend x m0.ctr h in
-        let m' : hmem_with_inv emp = inc_ctr m0 in
-        let h' : H.hheap (pts_to #a r x `star` linv m') = weaken _ (linv m0) (linv m') h' in
-        let m1 : hmem_with_inv (pts_to #a r x) = hmem_of_hheap m' h' in
+        let m' : hmem_with_inv_except e emp = inc_ctr m0 in
+        let h' : H.hheap (pts_to #a r x `star` linv e m') = weaken _ (linv e m0) (linv e m') h' in
+        let m1 : hmem_with_inv_except e (pts_to #a r x) = hmem_of_hheap m' h' in
         assert (forall frame. H.frame_related_heaps h h' emp (pts_to r x) frame true);
         let aux (frame:slprop)
           : Lemma
             (requires
-               interp ((emp `star` frame) `star` linv m0) m0)
+               interp ((emp `star` frame) `star` linv e m0) m0)
             (ensures
-               interp ((pts_to #a r x `star` frame) `star` linv m1) m1 /\
+               interp ((pts_to #a r x `star` frame) `star` linv e m1) m1 /\
                (forall (mp:mprop frame). mp (core_mem m0) == mp (core_mem m1)))
             [SMTPat (emp `star` frame)]
-          = star_associative emp frame (linv m0);
-            assert (H.interp (emp `star` (frame `star` linv m0)) h);
-            assert (H.interp (pts_to #a r x `star` (frame `star` linv m0)) h');
-            star_associative (pts_to #a r x) frame (linv m0);
-            assert (H.interp ((pts_to #a r x `star` frame) `star` linv m0) h');
-            assert (H.stronger (linv m0) (linv m'));
-            assert (H.equiv (linv m') (linv m1));
-            assert (H.stronger (linv m0) (linv m1));
-            let h' : H.hheap ((pts_to #a r x `star` frame) `star` linv m1) = weaken _ (linv m0) (linv m1) h' in
-            assert (H.interp ((pts_to #a r x `star` frame) `star` linv m1) h');
+          = star_associative emp frame (linv e m0);
+            assert (H.interp (emp `star` (frame `star` linv e m0)) h);
+            assert (H.interp (pts_to #a r x `star` (frame `star` linv e m0)) h');
+            star_associative (pts_to #a r x) frame (linv e m0);
+            assert (H.interp ((pts_to #a r x `star` frame) `star` linv e m0) h');
+            assert (H.stronger (linv e m0) (linv e m'));
+            assert (H.equiv (linv e m') (linv e m1));
+            assert (H.stronger (linv e m0) (linv e m1));
+            let h' : H.hheap ((pts_to #a r x `star` frame) `star` linv e m1) = weaken _ (linv e m0) (linv e m1) h' in
+            assert (H.interp ((pts_to #a r x `star` frame) `star` linv e m1) h');
             assert (forall (mp:H.hprop frame). mp h == mp h');
             mprop_preservation_of_hprop_preservation frame m0 m1;
             assert (forall (mp:mprop frame). mp (core_mem m0) == mp (core_mem m1))
         in
-        assert (frame_related_mems emp (pts_to r x) m0 m1);
+        assert (frame_related_mems emp (pts_to r x) e m0 m1);
         (| r, m1 |)
     in
-    refined_pre_action_as_action f
+    lift_tot_action (refined_pre_action_as_action f)
